WIP

new/proof/github_com/goose_lang/goose/model/channel/chan_spec_inv.v
@@ -7,48 +7,77 @@ Require Import New.proof.sync.
 Section proof.
  Context `{hG: heapGS Σ, !ffi_semantics _ _}. 
 Context `{!closePropTrackerG Σ,  !inG Σ (authR (optionUR (prodR fracR natR)))}.
+
 Implicit Types (v:val). 
 Context `{!ghost_varG Σ (bool * val)}.
 
-Record chan := {
-  ch_T': Type;
+
+
+Record chan  (t': Type) := {
   ch_T: go_type;
-  ch_IntoVal: IntoVal ch_T';
-  ch_IntoValTyped: IntoValTyped ch_T' ch_T;
-  ch_Hbounded: BoundedTypeSize ch_T;
+  #[export]
+  ch_IntoVal:: IntoVal t';
+  #[export]
+  ch_IntoValTyped:: IntoValTyped t' ch_T;
+  #[export]
+  ch_Hbounded:: BoundedTypeSize ch_T;
   ch_loc: loc;
-  ch_names: chan_names;
+  ch_mu: loc;
+  ch_buff: slice.t;
+  ch_γ: chan_names;
   ch_size: Z;
   ch_is_single_party: bool;
   ch_q: Qp;
-  ch_Psingle: Z -> ch_T' -> iProp Σ;
-  ch_Pmulti: ch_T' -> iProp Σ;
+  ch_Psingle: Z -> t' -> iProp Σ;
+  ch_Pmulti: t' -> iProp Σ;
   ch_Qsingle: Z -> iProp Σ;
   ch_Qmulti: iProp Σ;
   ch_R: nat -> iProp Σ;
-  ch_Ri: nat -> iProp Σ;
 }.
+  Arguments ch_T {t'}.
+  Arguments ch_IntoVal {t'}.
+Arguments ch_T {t'} .
+Arguments ch_IntoVal {t'} .
+Arguments ch_IntoValTyped {t'} .
+Arguments ch_Hbounded {t'} .
+Arguments ch_loc {t'} .
+Arguments ch_mu {t'} .
+Arguments ch_buff {t'} .
+Arguments ch_γ {t'} .
+Arguments ch_size {t'} .
+Arguments ch_is_single_party {t'} .
+Arguments ch_q {t'} .
+Arguments ch_Psingle {t'} .
+Arguments ch_Pmulti {t'} .
+Arguments ch_Qsingle {t'} .
+Arguments ch_Qmulti {t'} .
+
+
 
 (* Args for a simple use of send for synchronization i.e. using Send to join a goroutine. 
  Enforces that a channel isn't closed using a always-False R predicate. 
  *)
-Definition make_unbuffered_params_simple_single_sync (t': Type)
+Definition make_unbuffered_params_simple_single_sync
+ (t': Type)
 (t: go_type)
 (iv: IntoVal t')
 (ivt: IntoValTyped t' t)
 (hb: BoundedTypeSize t)
 (ch: loc)
+(mu: loc)
+(buff: slice.t)
 (γ: chan_names)
 (Psingle: Z -> t' -> iProp Σ)
-: chan :=
+: chan t' :=
 {|
-  ch_T' := t';
   ch_T := t;
   ch_IntoVal := iv;
   ch_IntoValTyped := ivt;
   ch_Hbounded := hb;
   ch_loc := ch;
-  ch_names := γ;
+  ch_mu := mu;
+  ch_buff := buff;
+  ch_γ := γ;
   ch_size := 0;
   ch_is_single_party := true;
   ch_q := 1%Qp;
@@ -57,7 +86,6 @@ Definition make_unbuffered_params_simple_single_sync (t': Type)
   ch_Qsingle := λ _, True%I;   
   ch_Qmulti := True%I;         
   ch_R := λ _,False%I; (*No closing*)
-  ch_Ri := λ _, False%I; (*No closing*)
 |}
 .
 
@@ -77,28 +105,29 @@ Definition buff_size_inv (count : Z) (first : u64) (size : Z): iProp Σ :=
 Definition valid_elems {T'} (slice : list T') (first : u64) (count : u64) : list T' :=
   subslice (uint.nat first) (uint.nat first + uint.nat count) (slice ++ slice).
 
-Definition isBufferedChanLogical (params: chan) 
+Definition isBufferedChanLogical  {t': Type} 
+ (params: chan t'  ) 
   (vs: valid_chan_state) (send_count recv_count: nat) (count: Z) 
-  (first: u64) (xs: list params.(ch_T')) : iProp Σ := 
+  (first: u64) (xs: list t') : iProp Σ := 
   "%HCountMinus" ∷ ⌜count = (send_count - recv_count)⌝ ∗
-  "%HSizeLen" ∷ ⌜params.(ch_size) = length xs⌝ ∗
+  "%HSizeLen" ∷ ⌜ch_size params = length xs⌝ ∗
   "%HBuffSizeInv" ∷ buff_size_inv count first (length xs) ∗
   "HPs" ∷ ([∗ list] i↦x ∈ valid_elems xs first count, 
-            P params.(ch_is_single_party) (recv_count + i) x params.(ch_Psingle) params.(ch_Pmulti)) ∗ 
-  "HQs" ∷ big_sep_seq send_count (params.(ch_size) - count) 
-           (λ i, Q params.(ch_is_single_party) (i - params.(ch_size)) params.(ch_Qsingle) params.(ch_Qmulti)).
+            P params.(ch_is_single_party)  (recv_count + i) x params.(ch_Psingle) params.(ch_Pmulti)) ∗ 
+  "HQs" ∷ big_sep_seq send_count (params.(ch_size)- count) 
+           (λ i, Q (ch_is_single_party  params) (i - params.(ch_size)) params.(ch_Qsingle) params.(ch_Qmulti)).
 
-Definition isBufferedChan (params: chan ) 
+Definition isBufferedChan (t': Type)  (params: chan t' ) 
   (vs: valid_chan_state) (send_count recv_count: nat) (count: Z) 
-  (buff: slice.t) (first: u64) : iProp Σ := 
+  (first: u64) : iProp Σ := 
   let intoVal := params.(ch_IntoVal) in
   let T := params.(ch_T) in
   let IntoVal_inst := params.(ch_IntoVal) in
   let IntoValTyped_inst := params.(ch_IntoValTyped) in
   let Hbounded := params.(ch_Hbounded) in
-  ∃ (xs: list params.(ch_T')), 
+  ∃ (xs: list t'), 
     "HBuffSlice" ∷ own_slice 
-                     buff (DfracOwn 1) xs ∗
+                     params.(ch_buff) (DfracOwn 1) xs ∗
     isBufferedChanLogical params vs send_count recv_count count first xs.
 
 Definition chan_state_facts (vs: valid_chan_state) (send_count recv_count: nat) : iProp Σ :=
@@ -111,117 +140,173 @@ match vs with
   | Valid_closed => ⌜send_count = recv_count⌝
 end.
 
-Definition chan_state_resources (params: chan)
-  (vs: valid_chan_state) (send_count recv_count: nat) (v: params.(ch_T')) : iProp Σ :=
-  let intoVal := params.(ch_IntoVal) in
+Definition chan_state_resources (t': Type) (params: chan t')
+  (vs: valid_chan_state) (send_count recv_count: nat) (v: t') : iProp Σ :=
+    let _ : IntoVal t' := params.(ch_IntoVal) in
   match vs with
   | Valid_start => 
-    "Hextok" ∷ full_exchange_token params.(ch_names) (* Full token with default value *)
+      "Hextok" ∷ full_exchange_token params.(ch_γ)
   | Valid_receiver_ready => 
-    "Hextok" ∷ receiver_exchange_token params.(ch_names) ∗ (* Receiver initiated *)
-    "HQ" ∷ Q params.(ch_is_single_party) recv_count params.(ch_Qsingle) params.(ch_Qmulti)
+      "Hextok" ∷ receiver_exchange_token params.(ch_γ) ∗
+      "HQ" ∷ Q params.(ch_is_single_party) recv_count params.(ch_Qsingle) params.(ch_Qmulti)
   | Valid_sender_ready => 
-    "Hextok" ∷ sender_exchange_token params.(ch_names) #v ∗ (* Sender initiated *)
-    "HP" ∷ P params.(ch_is_single_party) send_count v params.(ch_Psingle) params.(ch_Pmulti)
+      "Hextok" ∷ sender_exchange_token params.(ch_γ) v ∗
+      "HP" ∷ P params.(ch_is_single_party) send_count v params.(ch_Psingle) params.(ch_Pmulti)
   | Valid_receiver_done => 
-    "Hextok" ∷ sender_exchange_token params.(ch_names) #v ∗ (* Receiver will complete *)
-    "HQ" ∷ Q params.(ch_is_single_party) send_count params.(ch_Qsingle) params.(ch_Qmulti)
+      "Hextok" ∷ sender_exchange_token params.(ch_γ) v ∗
+      "HQ" ∷ Q params.(ch_is_single_party) send_count params.(ch_Qsingle) params.(ch_Qmulti)
   | Valid_sender_done => 
-    "Hextok" ∷ receiver_exchange_token params.(ch_names) ∗  (* Sender will complete *)
-    "HP" ∷ P params.(ch_is_single_party) recv_count v params.(ch_Psingle) params.(ch_Pmulti)  
+      "Hextok" ∷ receiver_exchange_token params.(ch_γ) ∗
+      "HP" ∷ P params.(ch_is_single_party) recv_count v params.(ch_Psingle) params.(ch_Pmulti)
   | Valid_closed => emp
   end.
 
-Definition isUnbufferedChan (params: chan)
-(v: params.(ch_T')) (vs: valid_chan_state) (send_count recv_count: nat) : iProp Σ := 
-"%HUnBuffFacts" ∷ chan_state_facts vs send_count recv_count ∗
-chan_state_resources params vs send_count recv_count v.
 
-Definition isChanInner (params: chan) (buff: slice.t) : iProp Σ := 
-  let T' := params.(ch_T') in
-  let T := params.(ch_T) in
-  let IntoVal_inst := params.(ch_IntoVal) in
-  let IntoValTyped_inst := params.(ch_IntoValTyped) in
-  let Hbounded := params.(ch_Hbounded) in
-  ∃ (vs: valid_chan_state) (count: nat) (first: u64) (v: T') (send_count recv_count: nat),
+Definition isUnbufferedChan (t': Type) (params: chan t')
+(v: t') (vs: valid_chan_state) (send_count recv_count: nat) : iProp Σ := 
+"%HUnBuffFacts" ∷ chan_state_facts vs send_count recv_count ∗
+chan_state_resources t' params vs send_count recv_count v.
+
+Definition isChanInner (t': Type) (params: chan t'): iProp Σ := 
+  ∃ (vs: valid_chan_state) (count: nat) (first: u64) (v: t') (send_count recv_count: nat),
     (* Physical state *)
-    "value" ∷ params.(ch_loc) ↦s[(channel.Channel.ty T) :: "v"] v ∗ 
-    "first" ∷ params.(ch_loc) ↦s[(channel.Channel.ty T) :: "first"] first ∗
-    "count" ∷ params.(ch_loc) ↦s[(channel.Channel.ty T) :: "count"] (W64 count) ∗ 
-    "state" ∷ params.(ch_loc) ↦s[(channel.Channel.ty T) :: "state"] (valid_to_word vs) ∗ 
+    "value" ∷ params.(ch_loc) ↦s[(channel.Channel.ty params.(ch_T)) :: "v"] v ∗ 
+    "first" ∷ params.(ch_loc) ↦s[(channel.Channel.ty params.(ch_T)) :: "first"] first ∗
+    "count" ∷ params.(ch_loc) ↦s[(channel.Channel.ty params.(ch_T)) :: "count"] (W64 count) ∗ 
+    "state" ∷ params.(ch_loc) ↦s[(channel.Channel.ty params.(ch_T)) :: "state"] (valid_to_word vs) ∗ 
     
     (* Counter resources *)
-    "HSndCtrAuth" ∷ own_send_counter_auth params.(ch_names) send_count (send_ctr_frozen vs) ∗ 
-    "HRcvCtrAuth" ∷ own_recv_counter_auth params.(ch_names) recv_count (recv_ctr_frozen vs send_count recv_count) ∗ 
+    "HSndCtrAuth" ∷ own_send_counter_auth params.(ch_γ) send_count (send_ctr_frozen vs) ∗ 
+    "HRcvCtrAuth" ∷ own_recv_counter_auth params.(ch_γ) recv_count (recv_ctr_frozen vs send_count recv_count) ∗ 
     
     (* Close resources *)
     "HCloseTokPostClose" ∷ 
       (match vs with
         | Valid_closed => 
            ∃ (n: nat) (close_tok_names: gset gname), 
-             own_closed_tok_post_close params.(ch_names) n close_tok_names ∗ 
-             own_send_counter_frag params.(ch_names) n 1
+             own_closed_tok_post_close params.(ch_γ) n close_tok_names ∗ 
+             own_send_counter_frag params.(ch_γ) n 1
         | _ => True
        end) ∗
 
     (* Buffer vs unbuffered channels *)
     "HChanState" ∷ 
       (if params.(ch_size) =? 0 then
-        isUnbufferedChan params v vs send_count recv_count
+        isUnbufferedChan t' params v vs send_count recv_count
       else
-        isBufferedChan params vs send_count recv_count count buff first).
+        isBufferedChan t' params vs send_count recv_count count first).
 
-Definition isChan (params: chan) : iProp Σ := 
-  let T' := params.(ch_T') in
-  let T := params.(ch_T) in
-  let IntoVal_inst := params.(ch_IntoVal) in
-  let IntoValTyped_inst := params.(ch_IntoValTyped) in
-  let Hbounded := params.(ch_Hbounded) in
-  ∃ (mu_l: loc) (buff: slice.t),
-    "#mu" ∷ params.(ch_loc) ↦s[(channel.Channel.ty T) :: "lock"]□ mu_l ∗
-    "#buffer" ∷ params.(ch_loc) ↦s[(channel.Channel.ty T) :: "buffer"]□ buff ∗
-    "%Hbuffsize" ∷ ⌜#buff.(slice.len_f) = #(W64 params.(ch_size))⌝ ∗
-    "#Hlock" ∷ is_Mutex mu_l (isChanInner params buff).
+Definition isChanInnerClosed (params: chan t'): iProp Σ := 
 
-Definition send_pre (params: chan) (i: nat) (v: params.(ch_T')) : iProp Σ :=
+  ∃ (count: nat) (first: u64) (v: t') (send_count recv_count: nat),
+    (* Physical state *)
+    "value" ∷ params.(ch_loc) ↦s[(channel.Channel.ty T) :: "v"] v ∗ 
+    "first" ∷ params.(ch_loc) ↦s[(channel.Channel.ty T) :: "first"] first ∗
+    "count" ∷ params.(ch_loc) ↦s[(channel.Channel.ty T) :: "count"] (W64 count) ∗ 
+    "state" ∷ params.(ch_loc) ↦s[(channel.Channel.ty T) :: "state"] (valid_to_word Valid_closed) ∗ 
+    
+    (* Counter resources *)
+    "HSndCtrAuth" ∷ own_send_counter_auth params.(ch_γ) send_count (send_ctr_frozen Valid_closed) ∗ 
+    "HRcvCtrAuth" ∷ own_recv_counter_auth params.(ch_γ) recv_count (recv_ctr_frozen Valid_closed send_count recv_count) ∗ 
+    
+    (* Close resources *)
+    "HCloseTokPostClose" ∷ 
+      
+           ∃ (n: nat) (close_tok_names: gset gname), 
+             own_closed_tok_post_close params.(ch_γ) n close_tok_names ∗ 
+             own_send_counter_frag params.(ch_γ) n 1
+         ∗
+
+    (* Buffer vs unbuffered channels *)
+    "HChanState" ∷ 
+      (if params.(ch_size) =? 0 then
+        isUnbufferedChan params v Valid_closed send_count recv_count
+      else
+        isBufferedChan params Valid_closed send_count recv_count count first).
+
+Definition isChan (params: chan t') : iProp Σ := 
+    "#mu" ∷ params.(ch_loc) ↦s[(channel.Channel.ty T) :: "lock"]□ params.(ch_mu) ∗
+    "#buffer" ∷ params.(ch_loc) ↦s[(channel.Channel.ty T) :: "buffer"]□ params.(ch_buff) ∗
+    "%Hbuffsize" ∷ ⌜#params.(ch_buff).(slice.len_f) = #(W64 params.(ch_size))⌝ ∗
+    "%Hbuffsize" ∷ ⌜0 ≤  params.(ch_size)⌝ ∗
+    "%Hbuffsize" ∷ ⌜params.(ch_size) + 1 < 2 ^ 63⌝ ∗
+    "#Hlock" ∷ is_Mutex params.(ch_mu) (isChanInner params).
+
+Definition send_pre (params: chan t') (i: nat) (v: t') : iProp Σ :=
   "%HChNonnull" ∷ ⌜params.(ch_loc) ≠ null⌝ ∗
   "%Hsp" ∷ ⌜if params.(ch_is_single_party) then params.(ch_q) = 1%Qp else (params.(ch_q) < 1)%Qp⌝ ∗
   "HCh" ∷ isChan params ∗
   "HP" ∷ P params.(ch_is_single_party) i v params.(ch_Psingle) params.(ch_Pmulti) ∗ 
-  "HSc" ∷ own_send_counter_frag params.(ch_names) i params.(ch_q).
+  "HSc" ∷ own_send_counter_frag params.(ch_γ) i params.(ch_q).
 
-Definition send_post (params: chan) (i: nat) : iProp Σ :=
+Definition send_pre_inner (params: chan t') (i: nat) (v: t') : iProp Σ :=
+  "%HChNonnull" ∷ ⌜params.(ch_loc) ≠ null⌝ ∗
+  "%Hsp" ∷ ⌜if params.(ch_is_single_party) then params.(ch_q) = 1%Qp else (params.(ch_q) < 1)%Qp⌝ ∗
+  "HCh" ∷ isChanInner params ∗
+  "%Hbuffsize" ∷ ⌜params.(ch_buff).(slice.len_f) = (W64 params.(ch_size))⌝ ∗
+    "#buffer" ∷ params.(ch_loc) ↦s[(channel.Channel.ty params.(ch_T)) :: "buffer"]□ params.(ch_buff) ∗
+  "HP" ∷ P params.(ch_is_single_party) i v params.(ch_Psingle) params.(ch_Pmulti) ∗ 
+  "HSc" ∷ own_send_counter_frag params.(ch_γ) i params.(ch_q).
+
+Definition send_post (params: chan t') (i: nat) : iProp Σ :=
 Q params.(ch_is_single_party) (i - params.(ch_size)) params.(ch_Qsingle) params.(ch_Qmulti) ∗ 
-own_send_counter_frag params.(ch_names) (i + 1)%nat params.(ch_q).
+own_send_counter_frag params.(ch_γ) (i + 1)%nat params.(ch_q).
 
-Definition recv_pre (params: chan) (i: nat) : iProp Σ :=
+
+Definition send_post_inner(params: chan t') (i: nat) : iProp Σ :=
+  "HCh" ∷ isChanInner params ∗
+Q params.(ch_is_single_party) (i - params.(ch_size)) params.(ch_Qsingle) params.(ch_Qmulti) ∗ 
+own_send_counter_frag params.(ch_γ) (i + 1)%nat params.(ch_q).
+
+Definition recv_pre (params: chan t') (i: nat) (Ri: nat -> iProp Σ) : iProp Σ :=
   "%HChnonnull" ∷ ⌜params.(ch_loc) ≠ null⌝ ∗
   "%Hsp" ∷  ⌜if params.(ch_is_single_party) then params.(ch_q) = 1%Qp else (params.(ch_q) < 1)%Qp⌝ ∗
   "HCh" ∷ isChan params ∗
   "HQ" ∷ Q params.(ch_is_single_party) i params.(ch_Qsingle) params.(ch_Qmulti) ∗ 
-  "HRecvPerm" ∷ own_recv_perm params.(ch_names) params.(ch_q) i params.(ch_Ri).
+  "HRecvPerm" ∷ own_recv_perm params.(ch_γ) params.(ch_q) i Ri.
 
-Definition default_val (params: chan) : params.(ch_T') :=
-@default_val params.(ch_T') params.(ch_T) _ params.(ch_IntoVal) params.(ch_IntoValTyped).
+Definition default_val (params: chan t') : t' :=
+@default_val t' params.(ch_T) _ params.(ch_IntoVal) params.(ch_IntoValTyped).
 
-Definition recv_post (params: chan) (i: nat) (ok: bool) (v: params.(ch_T')) : iProp Σ :=
+Definition recv_post (params: chan t') (i: nat) (ok: bool) (v: t') (Ri: nat -> iProp Σ) : iProp Σ :=
 if ok then
   (P params.(ch_is_single_party) i v params.(ch_Psingle) params.(ch_Pmulti) ∗ 
-   own_recv_perm params.(ch_names) params.(ch_q) (i + 1) params.(ch_Ri))%I
+   own_recv_perm params.(ch_γ) params.(ch_q) (i + 1) Ri)%I
 else
-  ("HRecFrag" ∷ own_recv_counter_frag params.(ch_names) i params.(ch_q) ∗ 
+  ("HRecFrag" ∷ own_recv_counter_frag params.(ch_γ) i params.(ch_q) ∗ 
    "%Hvdef" ∷ ⌜v = default_val params⌝ ∗ 
-   (∃ n, "HRi" ∷ params.(ch_Ri) n ∗ 
-         "#Hsca" ∷ own_send_counter_auth params.(ch_names) n true ∗ 
-         "#Hrca" ∷ own_recv_counter_auth params.(ch_names) n true))%I.
+   (∃ n, "HRi" ∷ Ri n ∗ 
+         "#Hsca" ∷ own_send_counter_auth params.(ch_γ) n true ∗ 
+         "#Hrca" ∷ own_recv_counter_auth params.(ch_γ) n true))%I.
 
-Lemma closed_unbuff_eq (params: chan) (send_count recv_count: nat) (v: params.(ch_T')):
+Definition recv_pre_inner (params: chan t') (i: nat) (Ri: nat -> iProp Σ) : iProp Σ :=
+"%HChnonnull" ∷ ⌜params.(ch_loc) ≠ null⌝ ∗
+"%Hsp" ∷ ⌜if params.(ch_is_single_party) then params.(ch_q) = 1%Qp else (params.(ch_q) < 1)%Qp⌝ ∗
+"HCh" ∷ isChanInner params ∗
+"%Hbuffsize" ∷ ⌜params.(ch_buff).(slice.len_f) = W64 params.(ch_size)⌝ ∗
+"#buffer" ∷ params.(ch_loc) ↦s[(channel.Channel.ty params.(ch_T)) :: "buffer"]□ params.(ch_buff) ∗
+"HQ" ∷ Q params.(ch_is_single_party) (Z.of_nat i) params.(ch_Qsingle) params.(ch_Qmulti) ∗ 
+"HRecvPerm" ∷ own_recv_perm params.(ch_γ) params.(ch_q) i Ri.
+       
+Definition recv_post_inner (params: chan t') (i: nat) (ok: bool) (v: t') (Ri: nat -> iProp Σ) : iProp Σ :=
+  "HCh" ∷ isChanInner params ∗
+  if ok then
+    (P params.(ch_is_single_party) (Z.of_nat i) v params.(ch_Psingle) params.(ch_Pmulti) ∗ 
+    own_recv_perm params.(ch_γ) params.(ch_q) (i + 1) Ri)%I
+  else
+    ("HRecFrag" ∷ own_recv_counter_frag params.(ch_γ) i params.(ch_q) ∗ 
+    "%Hvdef" ∷ ⌜v = default_val params⌝ ∗ 
+    (∃ n, "HRi" ∷ Ri n ∗ 
+          "#Hsca" ∷ own_send_counter_auth params.(ch_γ ) n true ∗ 
+          "#Hrca" ∷ own_recv_counter_auth params.(ch_γ) n true))%I.
+
+Lemma closed_unbuff_eq (params: chan t') (send_count recv_count: nat) (v: t'):
   isUnbufferedChan params v Valid_closed send_count recv_count -∗ ⌜send_count = recv_count⌝.
 Proof.
   iIntros "[%Heq _]". iPureIntro. exact Heq.
 Qed.
 
-Lemma chan_pointsto_non_null (lock: loc) (params: chan):
+Lemma chan_pointsto_non_null (lock: loc) (params: chan t'):
   params.(ch_loc) ↦s[channel.Channel.ty params.(ch_T) :: "lock"]□ lock -∗ ⌜ #params.(ch_loc) ≠ #null ⌝.
 Proof.
   iIntros "Hb.a".
