new/proof/github_com/goose_lang/goose/model/channel/chan_spec_api.v
@@ -1,8 +1,11 @@
 From New.proof.github_com.goose_lang Require Import primitive.
 From New.proof.github_com.goose_lang.std Require Import std_core.
-From New.proof.github_com.goose_lang.goose.model.channel Require Import chan_spec_inv chan_spec_select chan_spec_base.
+From New.proof.github_com.goose_lang.goose.model.channel Require Import chan_spec_inv chan_spec_select chan_spec_base chan_spec_send.
 From New.generatedproof.github_com.goose_lang.goose Require Import model.channel.
 From New.proof Require Import proof_prelude.
+Require Export New.code.sync.
+Require Export New.generatedproof.sync.
+From New.proof.sync_proof Require Import base mutex sema.
 
 
 Section proof.
@@ -12,7 +15,7 @@ Context `{!closePropTrackerG Σ,  !inG Σ (authR (optionUR (prodR fracR natR)))}
 Context `{!ghost_varG Σ (bool * val)}.
 #[global] Program Instance : IsPkgInit channel := ltac2:(build_pkg_init ()).
 
-Lemma wp_Channel__Send (params: chan) (i: nat) (v: params.(ch_T')):
+Lemma wp_Channel__Send  (params: chan) (i: nat) (v: params.(ch_T')):
 (* Could let bindings be implicit args? *)
   let T' := params.(ch_T') in
   let T := params.(ch_T) in
@@ -22,79 +25,52 @@ Lemma wp_Channel__Send (params: chan) (i: nat) (v: params.(ch_T')):
   params.(ch_loc) ≠ null ->
   (if params.(ch_is_single_party) then params.(ch_q) = 1%Qp else (params.(ch_q) < 1)%Qp) ->
   {{{ is_pkg_init channel ∗ send_pre params i v }}}
-    params.(ch_loc) @ channel @ "Channel'ptr" @ "Send" #T #v
+    params.(ch_loc) @ channel @ "Channel'ptr" @ "Send" #T #v 
   {{{ RET #();
       send_post params i
   }}}.
 Proof. 
   intros HT' HT Hiv_inst Hivt_inst Hb_inst Hnn Hsp. wp_start. wp_auto.   
-Admitted.
-
-Lemma wp_NewSendCase
-  (params: chan) (i: nat) (v: params.(ch_T')):
-  let T' := params.(ch_T') in
-  let T := params.(ch_T) in
-  let IntoVal_inst := params.(ch_IntoVal) in
-  let IntoValTyped_inst := params.(ch_IntoValTyped) in
-  let Hbounded := params.(ch_Hbounded) in
-  {{{ is_pkg_init channel ∗ send_pre params i v }}}
-    channel @ "NewSendCase" #T #params.(ch_loc) #v
-  {{{ (case_ptr: loc), RET #case_ptr;
-      own_select_case SelectSend params case_ptr false i (to_val v)
-  }}}.
-Proof.
-  intros HT' HT Hiv_inst Hivt_inst Hb_inst. wp_start. wp_auto.   iNamed "Hpre".
-  wp_apply wp_alloc. iIntros (ptr) "Hptr". 
-  iApply struct_fields_split in "Hptr"; iNamed "Hptr". wp_auto. iApply "HΦ".
-  iNamed "HCh".
-  unfold own_select_case. simpl.
-  destruct bool_decide.
+  let x := ident:(Φ) in
+  try clear x.
+ iNamed "Hpre". wp_if_destruct;first contradiction. wp_auto.
+  wp_apply (wp_NewSendCase with "[HCh HP c HSc]"). 
   {
-   done.
+    iFrame. iPureIntro. done.
   }
-  iFrame.  
-  iFrame.  simpl. iFrame "#". iPureIntro. done.
-Qed.
-
-Lemma wp_NewRecvCase
-  (params: chan) (i: nat):
-  let T' := params.(ch_T') in
-  let T := params.(ch_T) in
-  let IntoVal_inst := params.(ch_IntoVal) in
-  let IntoValTyped_inst := params.(ch_IntoValTyped) in
-  let Hbounded := params.(ch_Hbounded) in
-  {{{ is_pkg_init channel ∗ recv_pre params i }}}
-    channel @ "NewRecvCase" #T #params.(ch_loc)
-  {{{ (case_ptr: loc), RET #case_ptr;
-      own_select_case SelectRecv params case_ptr false i (to_val (default_val T'))
-  }}}.
-Proof.
-  intros HT' HT Hiv_inst Hivt_inst Hb_inst. wp_start. wp_auto. iNamed "Hpre".
-  wp_apply wp_alloc. iIntros (ptr) "Hptr".
-  iApply struct_fields_split in "Hptr"; iNamed "Hptr". wp_auto. iApply "HΦ".
-  iNamed "HCh".
-  unfold own_select_case. simpl.
-  destruct bool_decide.
+  iIntros (case_ptr) "Hosc". wp_auto. wp_apply (wp_Select1 with "[Hosc]").
   {
     done.
   }
-  iFrame.
-  simpl. iFrame "#". iPureIntro. done.
+  {
+    iFrame.
+  }
+  iIntros (selected_idx) "Hosc".
+  wp_auto. 
+  destruct selected_idx.
+  {
+   simpl. 
+   unfold own_select_case. 
+    iApply "HΦ". iFrame.
+    destruct bool_decide.
+    {
+      iDestruct "Hosc" as "[Ht Hf]".
+      done.
+    } unfold own_select_case_logical.
+    iNamed "Hosc".
+    iFrame.
+    iNamed "Hosc". iFrame.
+  }
+  iApply "HΦ".
+  unfold own_select_case.
+  destruct bool_decide eqn: Hb.
+  {
+    rewrite bool_decide_eq_true in Hb.
+    done.
+  }
+  iNamed "Hosc".
+  iDestruct "Hb" as "%". done.
 Qed.
-
-Lemma wp_Select1
-    (params1: chan)
-    (dir1: select_dir)
-    (case1 : loc)
-    (i1: nat) (v1: val)
-    (blocking : bool) :
-    {{{ is_pkg_init channel ∗ own_select_case dir1 params1 case1 false i1 v1 }}}
-      channel @ "Select1" #params1.(ch_T) #case1 #blocking
-    {{{ (selected_idx : nat), RET #(W64 selected_idx);
-        own_selected_case_params1 dir1 params1 blocking selected_idx case1 v1 i1 }}}.
-  Proof. 
-    wp_start. wp_auto.
-Admitted.
 
 Lemma wp_Channel__Receive (params: chan) (i: nat):
   (if params.(ch_is_single_party) then params.(ch_q) = 1%Qp else (params.(ch_q) < 1)%Qp) ->
@@ -113,62 +89,25 @@ Proof.
   {
     iFrame. iPureIntro. done.
   }
-  iIntros (case_ptr) "Hosc". wp_auto. wp_apply (wp_Select1 with "[Hosc]").
-  {
-   iFrame. 
-  }
+  iIntros (case_ptr) "Hosc". wp_auto. wp_apply (wp_Select1 with "[Hosc]"). all: try done.
   iIntros (selected_idx) "Hosc".
-  wp_auto. unfold own_selected_case_params1. iNamed "Hosc".
-  unfold own_selected_case_multi.
+  wp_auto.
+  iNamed "Hosc".
   destruct selected_idx.
   {
    simpl. 
-   unfold own_select_case. unfold nil_select_case. simpl.
+   unfold own_select_case. 
    iNamed "Hosc". 
    destruct bool_decide.
    {
     done.
    }
    iFrame.
+   iNamed "Hosc".
  
-   iNamed "Hselcase".
    wp_auto. iApply "HΦ". iFrame.
   }
-  destruct selected_idx.
-  {
-   simpl. 
-   unfold own_select_case. unfold nil_select_case. simpl.
-   iNamed "Hosc". iFrame. done.
-  }
-  destruct selected_idx.
-  {
-   simpl. 
-   unfold own_select_case. unfold nil_select_case. simpl.
-   iNamed "Hosc". iFrame. done.
-  }
-  destruct selected_idx.
-  {
-   simpl. 
-   unfold own_select_case. unfold nil_select_case. simpl.
-   iNamed "Hosc". iFrame. done.
-  }
-  destruct selected_idx.
-  {
-   simpl. 
-   unfold own_select_case. unfold nil_select_case. simpl.
-   iNamed "Hosc". iFrame. done.
-  }
-  destruct selected_idx.
-  {
-   simpl. 
-   unfold own_select_case. unfold nil_select_case. simpl.
-   iNamed "Hosc". iFrame. iDestruct "Hosc" as "[%Hosc %Hcontra]". done.  
-  }
-  simpl. destruct bool_decide eqn: Hc.
-  {
-    rewrite bool_decide_eq_true in Hc. lia.
-  }
-   iNamed "Hosc". iFrame. iDestruct "Hosc" as "[%Hosc %Hcontra]". done.  
+  iDestruct "Hb" as "%". done.
 Qed.
 
 Lemma wp_Channel__ReceiveDiscardOk (params: chan) (i: nat):
@@ -196,17 +135,21 @@ Proof.
 Qed.
 
 Lemma wp_NewChannelRef
-  (params: chan):
-  let T' := params.(ch_T') in
-  let T := params.(ch_T) in
-  let IntoVal_inst := params.(ch_IntoVal) in
-  let IntoValTyped_inst := params.(ch_IntoValTyped) in
-  let Hbounded := params.(ch_Hbounded) in
+ (t': Type)
+  (t: go_type)
+(iv: IntoVal t')
+(ivt: IntoValTyped t' t)
+(hb: BoundedTypeSize t)
+(Psingle: Z -> t' -> iProp Σ)
+(size: Z)
+
+:
+ 0 ≤ size ->
   {{{ is_pkg_init channel }}}
-    channel @ "NewChannelRef" #T #(W64 params.(ch_size))
+    channel @ "NewChannelRef" #t #(W64 0)
   {{{ (ch_ref_ptr: loc), RET #ch_ref_ptr;
-      ∃ 
-         (γ: chan_names),
+  ∃ (params:chan),
+          "%Hsize" ∷ ⌜params.(ch_size) = 0 ⌝ ∗ 
           "%Hchptr" ∷ ⌜params.(ch_loc) = ch_ref_ptr⌝ ∗
           "%Hchq" ∷ ⌜params.(ch_q) = 1%Qp⌝  ∗
           "HCh" ∷ isChan params ∗ 
@@ -214,92 +157,445 @@ Lemma wp_NewChannelRef
           "HRecvPerm" ∷ own_recv_perm params.(ch_names) params.(ch_q) 0 params.(ch_Ri)
   }}}.
 Proof.
-  intros HT' HT Hiv_inst Hivt_inst Hb_inst. wp_start. wp_auto.
-Admitted.
+  intros Hsz.
+   wp_start. wp_auto.
+  rewrite -wp_fupd.
+  wp_apply wp_slice_make2.
+  iIntros (slice) "Hslice".
+  wp_auto.
+  wp_alloc mu as "Hl".
+  wp_auto.
+  rewrite /named.
+  wp_alloc loc as "HCh".
+
+  iDestruct (struct_fields_split with "HCh") as "HCh".
+  iNamed "HCh". simpl.
+  iDestruct own_chan_ghost_alloc as ">H".
+  iNamed "H".
+  iDestruct "H" as "(Hscauth & Hscf & Hrcauth & Hrperm & Hoct &Het)".
+  pose my_params := make_unbuffered_params_simple_single_sync t' t iv ivt hb loc mu slice γ Psingle
+  .
+  iPersist "Hlock" as "#mu".
+  iPersist "Hbuffer" as "#buff".
+    
+
+  iDestruct "Hslice" as "[Hsl1 Hsl2]".
+  iDestruct (own_slice_len with "Hsl1") as "%Hlen".
+
+  iMod (init_Mutex (isChanInner my_params) _ mu
+         with "[$] [-HΦ Hscf Hrperm]") as "#Hlock".
+         {
+iModIntro.
+  unfold isChan. iFrame.
+  iFrame "#". 
+  unfold isChan. iFrame.
+  iFrame "#".
+  unfold make_unbuffered_params_simple_single_sync in my_params.
+  simpl in my_params.
+    replace my_params.(ch_buff) with slice in Hlen by done.
+  replace (my_params.(ch_size)) with 0 by set_solver.
+  simpl. rewrite length_replicate in Hlen.
+   replace (W64 0) with (slice .(slice.len_f)) by word.
+   iExists Valid_start. iFrame. iExists 0%nat.
+   replace (slice.(slice.len_f)) with (W64 0) by word.
+   iFrame. unfold isUnbufferedChan.
+   unfold chan_state_resources.
+   unfold chan_state_facts. simpl. 
+   iFrame.
+   done.
+  }
+
+  wp_auto_lc 2.
+  iModIntro.
+  iApply "HΦ".
+  replace mu with (my_params.(ch_mu)) by set_solver.
+  replace slice with (my_params.(ch_buff)) by set_solver.
+  iFrame "#".
+  replace (my_params.(ch_size)) with 0 by set_solver.
+  simpl. 
+  rewrite length_replicate in Hlen.
+    replace my_params.(ch_buff) with slice in Hlen by done.
+   replace (W64 0) with (slice .(slice.len_f)) by word.
+  iSplitL "".
+  {
+   done. 
+  }
+  iFrame.
+  iPureIntro. 
+   done.
+Qed.
+
+(* Len *)
+Lemma wp_Channel__Len_params (params: chan):
+  {{{ is_pkg_init channel ∗  isChan params }}}
+    params.(ch_loc) @ channel @ "Channel'ptr" @ "Len" #params.(ch_T) #()
+  {{{ (n: nat), RET #(W64 n); ⌜ (0 ≤ n)%nat ⌝ }}}.
+Proof.
+  wp_start. wp_auto. iNamed "Hpre".  wp_if_destruct.
+  {
+   iSpecialize ("HΦ" $! 0%nat).
+   iApply "HΦ". done. 
+  }
+  wp_auto.
+  wp_apply (wp_Mutex__Lock with "[$Hlock]").
+  iIntros "[Hlocked HisChanInner]". wp_pures.
+  iNamed "HisChanInner".
+  wp_auto.
+  wp_apply (wp_Mutex__Unlock with "[-chan_len HΦ]").
+  - iFrame. iFrame "#". iModIntro. iFrame.
+  - iApply "HΦ". iPureIntro. lia.
+Qed.
+
+(* Cap *)
+Lemma wp_Channel__Cap_params (params: chan):
+  params.(ch_loc) ≠ null ->
+  {{{ is_pkg_init channel ∗ isChan params }}}
+    params.(ch_loc) @ channel @ "Channel'ptr" @ "Cap" #params.(ch_T) #()
+  {{{ RET #(W64 params.(ch_size)); True%I }}}.
+Proof.
+  intros Hnn.
+  wp_start. wp_auto. iNamed "Hpre".  wp_if_destruct.
+  {
+    done.
+  }
+  {
+    wp_auto.
+    replace (params.(ch_buff).(slice.len_f)) with (W64 params.(ch_size)).
+    {
+       iApply "HΦ". done.
+    }
+    {
+       apply (inj _) in Hbuffsize.
+       done.
+    }
+  }
+Qed.
+
+
+(* Close *)
+Lemma wp_Channel__Close (params: chan) (n: nat) :
+  #params.(ch_loc) ≠ #null ->
+  {{{ is_pkg_init channel ∗ "HCh" ∷ isChan params ∗ "HCp" ∷ own_close_perm params.(ch_names) params.(ch_R) n }}}
+    params.(ch_loc) @ channel @ "Channel'ptr" @ "Close" #params.(ch_T) #()
+  {{{ RET #(); True }}}.
+Proof.
+  intros Hnotnull. wp_start. wp_auto.
+  wp_if_destruct. 
+  {
+   replace params.(ch_loc) with null in Hnotnull. exfalso. apply Hnotnull.
+   done. 
+  }
+  wp_auto.
+  iNamed "Hpre".
+  iAssert (∃ (done_b: bool),
+  "done" ∷  done_ptr ↦ done_b ∗ 
+  if done_b then True else 
+ ("HCh" ∷  isChan params ∗ 
+"HCp" ∷  own_close_perm params .(ch_names) params .(ch_R) n ∗ 
+"c" ∷  c_ptr ↦ params .(ch_loc) )%I )%I
+ with "[done HCh HCp c]" as "HI".
+ {
+  iExists false.
+  iFrame.
+ }
+  wp_for. 
+  iNamed "HI".
+   wp_auto.
+   destruct done_b.
+   {
+    destruct decide.
+    {
+      inversion e.
+      inversion H0.
+      assert (false = true) as Hcontra.
+      { apply (to_val_inj _ _ e). }
+      congruence. 
+      
+    }
+    destruct decide.
+    {
+     wp_auto. iApply "HΦ". done. 
+    }
+    done.
+   }
+   
+   destruct decide.
+   {
+    wp_auto.
+    iNamed "HI".
+   
+
+    simpl.
+      
+   iNamed "HCh".
+    
+   wp_auto.
+  wp_apply (wp_Mutex__Lock with "[$Hlock]").
+  iIntros "[Hlocked HisChanInner]". wp_auto.
+  wp_apply ((wp_Channel__TryClose) with "[$HisChanInner $HCp]").
+  {
+   done. 
+  } 
+  iIntros (selected) "IH". wp_auto.
+  iNamed "IH". 
+  destruct selected.
+  {
+  wp_apply (wp_Mutex__Unlock with "[$Hlocked IH $Hlock]").
+  {
+   iModIntro. 
+   {
+    iNamed "IH". unfold isChanInner. iFrame "value first count state".
+    iFrame "HSndCtrAuth HRcvCtrAuth".
+    iNamed "HCloseTokPostClose".
+    iDestruct "HCloseTokPostClose" as "(Hoc & Hscf & Hcs)".
+    iFrame.
+   } 
+  }
+  {
+    wp_for_post. iFrame.
+  }
+  }
+  iDestruct "IH" as "[Hcp IH]".
+  wp_apply (wp_Mutex__Unlock with "[$Hlocked  IH  $Hlock]").
+  {
+   iModIntro. 
+   {
+    iNamed "IH". unfold isChanInner.  iFrame "value first count state".
+    iFrame "HSndCtrAuth HRcvCtrAuth".
+    iNamed "HCloseTokPostClose".
+    destruct vs. all: try (iFrame;done).
+   }
+  } 
+   {
+    wp_for_post. iFrame "HΦ". iFrame. iFrame "#".
+    iSplitL "";first (iPureIntro;done).
+    iFrame.
+   }
+  }
+  {
+    done.
+  }
+Qed.
+
 
 Lemma wp_Select2
-    (dir1 dir2: select_dir)
-    (params1 params2: chan )
-    (case1 case2 : loc)
-    (blocking : bool) 
-  (v1 v2: val) 
-  (i1 i2: nat) : 
+(params1 params2: chan) 
+(dir1 dir2: select_dir)
+(case1_ptr case2_ptr: loc)
+(i1 i2: nat) 
+(v1: params1.(ch_T')) (v2: params2.(ch_T'))
+(blocking: bool):
+let T1 := params1.(ch_T) in
+let T2 := params2.(ch_T) in
+let IntoVal_inst1 := params1.(ch_IntoVal) in
+let IntoValTyped_inst1 := params1.(ch_IntoValTyped) in
+let IntoVal_inst2 := params2.(ch_IntoVal) in
+let IntoValTyped_inst2 := params2.(ch_IntoValTyped) in
+{{{ is_pkg_init channel ∗
+    own_select_case dir1 params1 case1_ptr false i1 #v1 ∗
+    own_select_case dir2 params2 case2_ptr false i2 #v2
+}}}
+  channel @ "Select2" #T1 #T2 #case1_ptr #case2_ptr #blocking
+{{{ (selected_idx: Z), RET #(W64 selected_idx);
+    ⌜selected_idx ≤ 2⌝ ∗
+    match selected_idx with 
+    | 0 =>
+      own_select_case dir1 params1 case1_ptr true i1 #v1 ∗
+      own_select_case dir2 params2 case2_ptr false i2 #v2
+    | 1 =>
+      own_select_case dir1 params1 case1_ptr false i1 #v1 ∗
+      own_select_case dir2 params2 case2_ptr true i2 #v2
+    | _ => 
+      ⌜blocking = false⌝ ∗
+      own_select_case dir1 params1 case1_ptr false i1 #v1 ∗
+      own_select_case dir2 params2 case2_ptr false i2 #v2
+      end
+}}}.
+intros Ht1 Ht2 Hiv1 Hivt1 Hiv2 Hivt2.
+wp_start. wp_auto. 
+iNamed "Hpre". 
+ wp_apply wp_alloc.
+iIntros (case_2) "Hc2p".
+wp_auto.
+wp_apply wp_alloc.
+iIntros (case_1) "Hc1p".
+wp_auto.
+wp_apply wp_RandomUint64.
+iIntros (x) "Hx". wp_auto.
+set ran := w64_word_instance .(word.modu) x (W64 2).
+set ind := uint.nat ran.
+assert (ind = uint.nat ran) by lia.
+assert (ind = 0%nat ∨ ind = 1%nat).
+{
+  destruct ind.
+  {
+   left. done. 
+  }
+  destruct ind.
+  {
+   right. done. 
+  }
+  subst ran.
+  word.
+}
+destruct ind eqn: Hin.
+{
+ assert (ran = (W64 0)) by word.
+wp_apply   (wp_TrySelectCase2 with "[Hpre]"). all: try done.
+{
+ left. done. 
+}
+iIntros (selected) "Hcases". 
+wp_auto. 
+destruct selected.
+{
+  wp_auto. replace ran with (W64 0). simpl. iApply "HΦ".
+  iFrame. done.
+}
+{
+ wp_auto. wp_for.
+    destruct decide.
+    {
+    iDestruct "Hcases" as "[H1 H2]".
+wp_apply   (wp_TrySelect with "[H1]"). all: try done.
+{
+iIntros (selected). rewrite H1.
+iIntros "Hcases". wp_auto. 
+destruct selected.
+{
+  wp_auto. wp_for_post. iApply "HΦ". iFrame. done.
+}
+{
+ wp_auto. 
+wp_apply   (wp_TrySelect with "[H2]"). all: try done.
+iIntros (selected).
+iIntros "Hcase2".
+ wp_auto. 
+destruct selected.
+{
+  wp_auto. wp_for_post. iApply "HΦ". iFrame. done.
+}
+{
+  wp_auto.
+  destruct blocking.
+  {
+    wp_auto. wp_for_post. iFrame. 
+  }
+  {
+   wp_auto. wp_for_post. iFrame. 
+   iApply "HΦ". iFrame. done.
+  }
+}
+}
+}
+    }
+{
+    iDestruct "Hcases" as "[H1 H2]".
+wp_apply   (wp_TrySelect with "[H1]"). all: try done.
+}
+}
+}
+{
+  wp_apply   (wp_TrySelectCase2 with "[Hpre]"). all: try done.
+{
+  word.
+}
+iIntros (selected) "Hcases". 
+wp_auto. 
+destruct selected.
+{
+  wp_auto. 
+   destruct n.
+  {
+  assert (ind = 1%nat) by lia.
+  assert (ran = (W64 1)) by word.
+  replace ran with (W64 1).
+  iApply "HΦ". iFrame. done.
+  }
+  {
+    replace ran with (W64 (S (S n))) by word.
+   iApply "HΦ". lia. 
+  }
+}
+{
+ wp_auto. wp_for.
+  destruct decide.
+    {
+    iDestruct "Hcases" as "[H1 H2]".
+wp_apply   (wp_TrySelect with "[H1]"). all: try done.
+{
+iIntros (selected). rewrite e.
+iIntros "Hcases". wp_auto. 
+destruct selected.
+{
+  wp_auto. wp_for_post. iApply "HΦ". iFrame. done.
+}
+{
+ wp_auto. 
+wp_apply   (wp_TrySelect with "[H2]"). all: try done.
+iIntros (selected).
+iIntros "Hcase2".
+wp_auto. 
+destruct selected.
+{
+ wp_auto. wp_for_post. iApply "HΦ". iFrame. done. 
+}
+{
+ wp_auto. 
+  destruct blocking.
+  {
+    wp_auto. wp_for_post. iFrame. 
+  }
+  {
+   wp_auto. wp_for_post. iFrame. 
+   iApply "HΦ". iFrame. done.
+  }
 
-    {{{ is_pkg_init channel ∗ own_select_case dir1 params1 case1 false i1 v1 ∗ own_select_case dir2 params2 case2 false i2 v2 }}}
-      channel @ "Select2" #params1.(ch_T) #params2.(ch_T) #case1 #case2 #blocking
-    {{{ (i : nat), RET #(W64 i);
-        own_selected_case_params2 dir1 dir2 params1 params2 blocking i case1 case2 v1 v2 i1 i2 }}}.
-    Proof.
-      wp_start. wp_auto.
-Admitted.
+}
 
-Lemma wp_Select3
-  (dir1 dir2 dir3: select_dir)
-  (params1 params2 params3: chan)
-  (case1 case2 case3: loc)
-  (blocking: bool)
-  (v1 v2 v3: val)
-  (i1 i2 i3: nat) :
-  {{{ is_pkg_init channel ∗
-      own_select_case dir1 params1 case1 false i1 v1 ∗
-      own_select_case dir2 params2 case2 false i2 v2 ∗
-      own_select_case dir3 params3 case3 false i3 v3 }}}
-    channel @ "Select3" #params1.(ch_T) #params2.(ch_T) #params3.(ch_T)
-                         #case1 #case2 #case3 #blocking
-  {{{ (i : nat), RET #(W64 i);
-      own_selected_case_params3 dir1 dir2 dir3 params1 params2 params3 blocking i
-                                case1 case2 case3 v1 v2 v3 i1 i2 i3 }}}.
-Proof.
-  wp_start. wp_auto.
-Admitted.
+} 
+}
+    }
+    {
+      iDestruct "Hcases" as "[H1 H2]".
+wp_apply   (wp_TrySelect with "[H1]"). all: try done.
+{
+iIntros (selected). 
+iIntros "Hcases". wp_auto. 
+destruct selected.
+{
+  wp_auto. wp_for_post. iApply "HΦ". iFrame. done.
+}
+{
+ wp_auto. 
+wp_apply   (wp_TrySelect with "[H2]"). all: try done.
+iIntros (selected).
+iIntros "Hcase2".
+wp_auto. 
+destruct selected.
+{
+ wp_auto. wp_for_post. iApply "HΦ". iFrame. done. 
+}
+{
+ wp_auto. 
+  destruct blocking.
+  {
+    wp_auto. wp_for_post. iFrame. 
+  }
+  {
+   wp_auto. wp_for_post. iFrame. 
+   iApply "HΦ". iFrame. done.
+  }
 
-Lemma wp_Select4
-  (dir1 dir2 dir3 dir4: select_dir)
-  (params1 params2 params3 params4: chan)
-  (case1 case2 case3 case4: loc)
-  (blocking: bool)
-  (v1 v2 v3 v4: val)
-  (i1 i2 i3 i4: nat) :
-  {{{ is_pkg_init channel ∗
-      own_select_case dir1 params1 case1 false i1 v1 ∗
-      own_select_case dir2 params2 case2 false i2 v2 ∗
-      own_select_case dir3 params3 case3 false i3 v3 ∗
-      own_select_case dir4 params4 case4 false i4 v4 }}}
-    channel @ "Select4" #params1.(ch_T) #params2.(ch_T) #params3.(ch_T) #params4.(ch_T)
-                         #case1 #case2 #case3 #case4 #blocking
-  {{{ (i : nat), RET #(W64 i);
-      own_selected_case_params4 dir1 dir2 dir3 dir4
-        params1 params2 params3 params4 blocking i
-        case1 case2 case3 case4 v1 v2 v3 v4 i1 i2 i3 i4 }}}.
-Proof.
-  wp_start. wp_auto.
-Admitted.
+}
 
-Lemma wp_Select5
-  (dir1 dir2 dir3 dir4 dir5: select_dir)
-  (params1 params2 params3 params4 params5: chan)
-  (case1 case2 case3 case4 case5: loc)
-  (blocking: bool)
-  (v1 v2 v3 v4 v5: val)
-  (i1 i2 i3 i4 i5: nat) :
-  {{{ is_pkg_init channel ∗
-      own_select_case dir1 params1 case1 false i1 v1 ∗
-      own_select_case dir2 params2 case2 false i2 v2 ∗
-      own_select_case dir3 params3 case3 false i3 v3 ∗
-      own_select_case dir4 params4 case4 false i4 v4 ∗
-      own_select_case dir5 params5 case5 false i5 v5 }}}
-    channel @ "Select5"
-             #params1.(ch_T) #params2.(ch_T) #params3.(ch_T) #params4.(ch_T) #params5.(ch_T)
-             #case1 #case2 #case3 #case4 #case5 #blocking
-  {{{ (i : nat), RET #(W64 i);
-      own_selected_case_params5 dir1 dir2 dir3 dir4 dir5
-        params1 params2 params3 params4 params5
-        blocking i
-        case1 case2 case3 case4 case5
-        v1 v2 v3 v4 v5
-        i1 i2 i3 i4 i5 }}}.
-Proof.
-  wp_start. wp_auto.
-Admitted.
+} 
+}
+      
+    }
+}
+}
+Qed.
+
 
 End proof.
